proof/crypto_scalarmult/curve25519/amd64/ref4/CryptolineEquivs_Ref4.ec
@@ -1,4 +1,4 @@
-require import Ref4_scalarmult_s Jcheck Add4Extracted Sub4Extracted Mul4RefExtracted Mul4_a24RefExtracted Int.
+require import Ref4_scalarmult_s Jcheck Add4Extracted Sub4Extracted Mul4RefExtracted Mul4_a24RefExtracted Int Sqr4RefExtracted.
 
 from Jasmin require import JWord.
 
@@ -10,8 +10,7 @@ proof.
     proc. 
     seq 9 14 : (={f, g, h, z} /\  _1{1} = cf{2}). by sim.
     seq 7 20 : (={f, g, h, z} /\ _2{1} = cf{2}). by sim.
-    seq 1 5 : (={f, g, h, z}). by sim. 
-    wp; skip; auto => />.
+    sim : (={f, g, h, z}). auto => />. 
     rewrite addcE /carry_add b2i0 => />. 
 qed.
 
@@ -21,8 +20,7 @@ proof.
     proc.  
     seq 9 14 : (={f, gs, h, z} /\  _1{1} = cf{2}). by sim.
     seq 7 16 : (={f, gs, h, z} /\ _2{1} = cf{2}). by sim.
-    seq 1 5 : (={f, gs, h, z}). by sim. 
-    wp; skip; auto => />.
+    sim : (={f, gs, h, z}). auto => />.
     rewrite subcE /borrow_sub b2i0 => />. 
 qed.
 
@@ -40,13 +38,27 @@ proof.
     rewrite !/mulhi !/mulu !addcE !/carry_add => />. 
 qed.
 
+lemma __reduce_cryptoline_equiv_sqr_ref4  :
+      equiv [Ref4_scalarmult_s.M.__reduce4 ~ Sqr4RefExtracted.M.__reduce4 : ={z} ==> res{1} = res{2}.`1].
+proof.
+    proc.
+    seq 36 52 : (={r, r38, rax, h, l, i, z, z8, cf}). by sim. 
+    seq 6 14 : (={r, r38, rax, h, l, i, z, z8, r0, cf}). auto => />.
+    rewrite !addcE !/carry_add !muluE !/mulhi => />. 
+    seq 2 2 : (={r, r38, rax, h, l, i, z8, z, r0, cf}). by sim.
+    sim : (={r, r38, rax, h, l, i, z8, r0, z}). auto => />.
+    move => *. do split. 
+    rewrite !/mulhi !/mulu !addcE !/carry_add => />. 
+    rewrite !/mulhi !/mulu !addcE !/carry_add => />. 
+qed.
+
+
 lemma __mul4_rss_cryptoline_equiv_ref4  :
       equiv [Ref4_scalarmult_s.M.__mul4_rss ~ Mul4RefExtracted.M.__mul4_rss : ={xa, ya} ==> res{1} = res{2}.`1].
 proof.
     proc.     
     wp. call __reduce_cryptoline_equiv_ref4.
-    seq 6 10 : (={x, y, z, r, xa, ya}). by sim. 
-    seq 3 3 : (={x, y, z, r, xa, ya}). by sim.
+    seq 9 13 : (={x, y, z, r, xa, ya}). by sim.
     unroll for{1} ^while. unroll for{2} ^while.
     seq 4 4 : (={x, y, z, r, xa, ya, hprev, i}).  
     unroll for{1} ^while. unroll for{2} ^while.
@@ -60,15 +72,22 @@ proof.
     wp. skip. auto => />.
 qed.
 
-
 lemma __mul4_a24_rs_cryptoline_equiv_ref4  :
-      equiv [Ref4_scalarmult_s.M.__mul4_a24_rs ~ Mul4_a24RefExtracted.M.__mul4_a24_rs : ={xa} /\ a24{1} = W64.of_int 121666 ==> res{1} = res{2}.`1].
+      equiv [Ref4_scalarmult_s.M.__mul4_a24_rs ~ Mul4_a24RefExtracted.M.__mul4_a24_rs : ={xa} /\ a24{1} = W64.of_int 121665 ==> res{1} = res{2}.`1].
 proof.
     proc. 
-    seq 7 15 : (={r, c, rax, rdx, xa}). auto => />.
-    seq 21 21 : (={r, c, rax, rdx, xa, t1, t2, t3, t4}). auto => />.
-    seq 15 23 : (={r, c, rax, rdx, xa, t1, t2, t3, t4, cf}). auto => />.
-    auto => />. 
-    move => &2. rewrite !addcE !/carry_add !b2i0  => />. 
+    seq 4 12 : (={r, c, rax, rdx, xa}). auto => />.
+    seq 39 47 : (={r, c, rax, rdx, xa, t1, t2, t3, t4, cf}). auto => />.
+    sim : (={r, c, rax, rdx, xa, t1, t2, t3, t4}). auto => />.
+    move => &2. rewrite !addcE !/carry_add !b2i0  => />.  
 qed.
+
+lemma __sqr4_rs_cryptoline_equiv_ref4  :
+      equiv [Ref4_scalarmult_s.M.__sqr4_rs ~ Sqr4RefExtracted.M.__sqr4_rs : ={xa} ==> res{1} = res{2}.`1].
+proof.
+    proc. 
+    wp. call __reduce_cryptoline_equiv_sqr_ref4.
+    sim : (={zero, xa, r, t, z, rax, rdx, aux, aux_0}). 
+qed.
+
 
